lean/Project.lean
@@ -2,6 +2,9 @@ import Project.BinarySearch.Pure
 import Project.BinarySearch.Rules
 import Project.BinarySearch.Program
 import Project.BinarySearch.Smoke
+import Project.BinarySearch.Spec
 import Project.BinarySearchOpt3.Program
 import Project.BinarySearchOpt3.Smoke
 import Project.BinarySearchOpt3.Equivalence
+import Project.BinarySearchOpt3.Spec
+import Project.BinarySearchOpt3.TotalProof
